we doen

2.dfy
@@ -14,36 +14,45 @@ function length<T>(l: List<T>): nat
   case Cons(_, t) => 1 + length(t)
 }
 
-function mem<T(==)> (x: T, l: List<T>) : bool
+function mem<T(==)> (x: T, n: nat, l: List<T>) : bool
+  requires n <= length(l)
 {
   match l
   case Nil => false
-  case Cons(head, t) => if(head == x)
-  then true
-  else
-    mem(x,t)
+  case Cons(y, t) =>
+    if(n == 0) then
+      if (y == x) then true
+      else
+        false
+    else
+      mem(x,n-1,t)
 }
-
 
 method from_array<T>(a: array<T>) returns (l: List<T>)
   requires a.Length >= 0
   ensures length(l) == a.Length
-  ensures forall i: int :: 0 <= i < a.Length ==> mem(a[i], l)
+  ensures forall i: int :: 0 <= i < a.Length ==> mem(a[i],i, l)
 
 {
   l := Nil;
   var i: int := a.Length - 1;
   while(i >= 0)
     invariant -1 <= i <= a.Length - 1
-    invariant forall j: int ::  i < j <= a.Length - 1 ==> mem(a[j], l)
     invariant length(l) == a.Length - 1 - i
+    invariant forall j: int :: i < j < a.Length ==> mem(a[j], j - i - 1, l)
   {
     l := Cons(a[i], l);
     i := i-1;
   }
 }
 
-method main() {
-  var l: List<int> := Cons(1, Nil);
-  assert length(l) == 1;
+method Main() {
+  var l: List<int> := List.Cons(1, List.Cons(2, List.Cons(3, Nil)));
+  var arr: array<int> := new int [3](i => i + 1);
+  var t: List<int> := from_array(arr);
+  print l;
+  print "\n";
+  print t;
+  print "\n";
+  print t == l;
 }
